### Exercise 9.10

$$ e ::= \cdots | \lambda x \cdots x . e | e(e, \cdots, e) $$

$$ v ::= \cdots | \langle \lambda x \cdots x.e, \sigma \rangle $$

$$ \sigma \vdash \lambda x_1, \cdots, x_n.e \implies \langle \lambda x_1, \cdots, x_n.e , \sigma \rangle $$

#### 1. Operational semantics of the form $\sigma \vdash e \implies v $

We only need define the inference rule of a function application rule in operational semantics.

For an expression $e_0 \quad e_1$, assume followings are given.

$$ \sigma \vdash e_0 \implies \langle \lambda x_1, \cdots, x_n . e, \sigma' \rangle $$

$$ \sigma \vdash e_i \implies v_i \quad (1 \le i \le n) $$

$$ \sigma' [ x_i \mapsto v_i \quad (1 \le i \le n) ] \vdash e \implies v $$

Then, we have

$$ \sigma \vdash e_0(e_1, \cdots, e_n) \implies v $$

#### 2. Write the evaluation derivation of $(\lambda \text{f m. f(m)})(\lambda x.x, 8)$

...
